%%
%% Author: semenovd
%% 27/02/2019
%%

% Preamble
\documentclass[11pt]{article}

% Packages
\usepackage{amsmath}
\usepackage{upgreek}
\usepackage{amsthm}
\usepackage{amssymb}

% Document
\begin{document}

   \pagenumbering{gobble}
   \paragraph{Task}\mbox{} \\
   Prove that for any natural number n,
   \begin{equation*}
      2 + 2^{2} + 2^{3} + 2^{4} + \mathellipsis + 2^{n} = 2^{n+1} - 2
   \end{equation*}
   \paragraph{Solution}\mbox{} \\
   Task is equavalent to proving the following theorem:
   \newtheorem*{Theorem}{Theorem}
   \begin{Theorem}
       $\displaystyle \forall n \in \mathbb{N}: \sum_{i=1}^{n}2^{n} = 2^{n+1} - 2$
   \end{Theorem}
   \begin{proof}
   By induction. \\
   \emph{Initial step (n = 1):} $\displaystyle \sum_{i=1}^{1}2^{1} = 2^{1+1} - 2$\\
   $\Rightarrow$ $2 = 4 - 2$ (by algebra)\\
   $\Rightarrow$ $2 = 2$, so equality holds.\\
   \emph{Induction step:} \\
   Assume $\displaystyle \sum_{i=1}^{n}2^{n} = 2^{n+1} - 2$. \\
   Then for $n + 1$: \\
   $\displaystyle \sum_{i=1}^{n + 1}2^{n + 1} = \sum_{i=1}^{n}2^{n} + 2^{n + 1}$ (pulling out last member)  \\
   $= 2^{n + 1} - 2 + 2^{n + 1}$ (by induction hypothesis)  \\
   $= 2\cdot2^{n + 1} - 2$ \\
   $= 2^{n + 2} - 2$. \\
   Thus $\displaystyle \sum_{i=1}^{n + 1}2^{n + 1} = 2^{n+2} - 2$, which is induction hypothesis for $n + 1$. \\
   Hence, by principle of induction,
   $\displaystyle \forall n \in \mathbb{N}: \sum_{i=1}^{n}2^{n} = 2^{n+1} - 2$
   \end{proof}

\end{document}